\documentclass[12pt]{article}
\usepackage{times}
\usepackage{graphicx}
\usepackage{graphics}
\usepackage{upgreek}
\usepackage{float}
\usepackage{epstopdf}
\usepackage{amsmath}
\usepackage{multicol, caption}
\usepackage{wrapfig}
\usepackage{amssymb}
\usepackage{pdflscape}
\usepackage{breqn}
\usepackage[margin=1in]{geometry}
\usepackage{tikz}
\usepackage{listings}
\usepackage{cite}


\newcommand{\hfd}{\hat{f}^{\delta}}
\newcommand{\tfd}{\tilde{f}^{\delta}}
\newcommand{\tfdp}{\tilde{f}^{\delta \prime}}
\newcommand{\hf}{\hat{f}}
\newcommand{\hfI}{\hat{f}^{\delta I}}
\newcommand{\hfC}{\hat{f}^{\delta C}}
\newcommand{\hfD}{\hat{f}^{\delta D}}
\newcommand{\bhfd}{\hat{\mathbf{f}}^{\delta}}
\newcommand{\btfd}{\tilde{\mathbf{f}}^{\delta}}

\newcommand{\hud}{\hat{u}^{\delta}}
\newcommand\hudi[1]{\hat{u}^{\delta(#1)}}
\newcommand{\tud}{\tilde{u}^{\delta}}
\newcommand{\tudp}{\tilde{u}^{\delta \prime}}
\newcommand{\bhud}{\hat{\mathbf{u}}^{\delta}}
\newcommand{\btud}{\tilde{\mathbf{u}}^{\delta}}
\newcommand{\bud}{\mathbf{u}^{\delta}}
\newcommand{\hu}{\hat{u}}
\newcommand{\huI}{\hat{u}^{\delta I}}
\newcommand{\huC}{\hat{u}^{\delta C}}

\newcommand\tb[1]{\tilde{\mathbf{#1}}}
\newcommand\hb[1]{\hat{\mathbf{#1}}}

\newcommand\px[2]{\frac{\partial #1}{\partial {#2}}}
\newcommand\pxi[3]{\frac{\partial^{#1}#2}{\partial {#3}^{#1}}}
\newcommand\dx[2]{\frac{\mathrm{d} #1}{\mathrm{d} #2}}
\newcommand\dxi[3]{\frac{\mathrm{d}^{#1}#2}{\mathrm{d} {#3}^{#1}}}
\newcommand\rint[2]{\int^{1}_{-1}{#1} \mathrm{d}{#2}}
\newcommand\poch[2]{({#1})_{#2}}

\newcommand\jump[1]{\llbracket{#1}\rrbracket}
\newcommand\mean[1]{\llbrace{#1}\rrbrace}
\newcommand\abracket[1]{\left\langle{#1}\right\rangle}
\newcommand\inprod[2]{\abracket{#1|#2}}
\newcommand{\half}{\frac{1}{2}}

\begin{document}

\title{Reference Equations}
\author{Will Trojak}

\maketitle



\section{Navier-Stokes}



\section{Maxwells' Equations}

	Base Maxwell's Equations
	\begin{align}
		\nabla \cdot \mathbf{B} &= 0\\
		\nabla \cdot \mathbf{E} &= \frac{\rho_c}{\epsilon_0} \\
		\frac{\partial \mathbf{B}}{\partial t} + \nabla \times \mathbf{E} &= 0 \\ 
		\frac{1}{\epsilon_0 \mu_0} \frac{\partial \mathbf{E}}{\partial t} - \nabla \times \mathbf{B} &= -\mu_0 \mathbf{j_c} 
	\end{align}

	A useful conversion is:
	\begin{equation}
		\mathrm{E} = \frac{\mathbf{D}}{\epsilon_0}	
	\end{equation}
	
	Casting the equation set into a CFD like conservative form:
	\begin{align}
		\frac{\partial \mathbf{Q}}{\partial t} + \nabla \cdot \mathbf{R(\mathbf{Q})} &= \mathbf{S} \\
		\mathbf{Q} = 
			\begin{bmatrix}
       			\mathbf{B} \\
       			\mathbf{D}
     		\end{bmatrix} \quad
     	\mathbf{R} &= \begin{bmatrix}
       			\mathbf{I} \times \mathbf{D}/\epsilon_0 \\
       		    -\mathbf{I} \times \mathbf{B}/\mu_0
     		\end{bmatrix} \quad
     	\mathbf{S} = \begin{bmatrix}
     			\mathbf{0} \\
       			-\mathbf{j}_c
     		\end{bmatrix}
	\end{align}		
	
	This can then be written as:
	\begin{align}
		\mathbf{Q}_t + \mathbf{F}_x + \mathbf{G}_y + \mathbf{H}_z &= \mathbf{S} \\
		\mathbf{F} = 
			\begin{bmatrix}
     			0 \\
     			-D_k/\epsilon \\
     			D_j/\epsilon \\
     			0 \\
     			B_k /\mu \\
     			-B_y/\mu
     		\end{bmatrix} \quad
     	\mathbf{G} &= 
			\begin{bmatrix}
     			D_k/\epsilon \\
     			0 \\
     			-D_i/\epsilon \\
     			-B_k /\mu \\
     			0\\
     			B_i/\mu
     		\end{bmatrix} \quad
     	\mathbf{H} = 
			\begin{bmatrix}
     			-D_j/\epsilon \\
     			D_i/\epsilon \\
				0 \\     			
     			B_j /\mu \\
     			-B_i/\mu \\
     			0
     		\end{bmatrix} \quad
	\end{align}
	
	If divergence cleaning is used then:
	\begin{align}
		\mathbf{Q} = 
			\begin{bmatrix}
       			\mathbf{B} \\
       			\mathbf{D} \\
       			\Phi \\
       			\Psi 
     		\end{bmatrix} \quad
     	\mathbf{R} &= \begin{bmatrix}
       			\mathbf{I} \times \mathbf{D}/\epsilon + \zeta \mathbf{I}\cdot \Psi\\
       		    -\mu \mathbf{I} \times \mathbf{B}/ + \chi \mu\mathbf{I}\cdot \Phi/ \\
       		    \chi \mathbf{E}\\
       		    \zeta\mu\mathbf{B}
     		\end{bmatrix} \quad
     	\mathbf{S} = \begin{bmatrix}
     			\mathbf{0} \\
       			-\mathbf{j}_c \\
       			\zeta \rho_c \\ 
       			0
     		\end{bmatrix}
	\end{align}
	and 
	\begin{align}
		\mathbf{Q}_t + \mathbf{F}_x + \mathbf{G}_y + \mathbf{H}_z &= \mathbf{S} \\
		\mathbf{F} = 
			\begin{bmatrix}
     			\zeta \Psi \\
     			-D_k/\epsilon \\
     			D_j/\epsilon \\
     			\chi \mu \Phi  \\
     			B_k /\mu \\
     			-B_y/\mu \\
     			\chi D_i/\epsilon \\
     			\zeta B_i/\mu
     		\end{bmatrix} \quad
     	\mathbf{G} &= 
			\begin{bmatrix}
     			D_k/\epsilon \\
     			\zeta \Psi \\
     			-D_i/\epsilon \\
     			-B_k /\mu \\
     			\chi \Phi\\
     			B_i/\mu \\
     			\chi D_j/\epsilon \\
     			\zeta B_j/\mu
     		\end{bmatrix} \quad
     	\mathbf{H} = 
			\begin{bmatrix}
     			-D_j/\epsilon \\
     			D_i/\epsilon \\
				\zeta \Psi \\     			
     			B_j /\mu \\
     			-B_i/\mu \\
     			\chi \Phi \\
     			\chi D_k/\epsilon \\
     			\zeta B_k /\mu
     		\end{bmatrix} \quad
	\end{align}

\section{Orthogonal Polynomials}

\begin{equation}
		\rint{\xi^nw(\xi)}{\xi} = \mu_n \quad \forall n\in\mathbb{N} \;\; \mathrm{and} \;\; \mu_n\in\mathbb{R}
	\end{equation}
	\begin{equation}
		\rint{P_iP_jw(\xi)}{\xi} = I^w_{i,j}, \quad  P_i,P_j\in P
	\end{equation}
	\begin{equation}
		P_{n+1} = (\xi - a_n)P_n - b_nP_{n-1}, \quad n=0,1,\dots
	\end{equation}

	\begin{align}
		a_n &= \frac{\inprod{\xi P_n}{P_n}}{\inprod{P_n}{P_n}}, \quad n\in\{0,1,\dots\}\\
		b_n &= \frac{\inprod{P_n}{P_n}}{\inprod{P_{n-1}}{P_{n-1}}}, \quad n\in\{1,2,\dots\}
	\end{align}

	\begin{equation}
		\inprod{f}{g} = \rint{f(\xi)g(\xi)w(\xi)}{\xi}.
	\end{equation}
	
\section{Flux Reconstruction}
	\begin{align}
		\hat{u} &= Ju \\
		\hat{\mathbf{f}} &= J\mathbf{G}^{-1}\mathbf{f} \\
		\hat{\nabla}\cdot\hat{\mathbf{f}} &= J \nabla\cdot\mathbf{f} \\
		\hat{\nabla}u &= \mathbf{G}\nabla u
	\end{align}
	
	\begin{equation}
		\mathbf{\Omega} = \bigcup^N_{n=1}\mathbf{\Omega}_n \quad \mathrm{and} \quad \bigcap^N_{n=1}\mathbf{\Omega}_n = \emptyset
	\end{equation}	
	\begin{equation}
		\mathbf{G}_n = \begin{bmatrix}
			\px{x_1}{\xi_1} & \px{x_2}{\xi_1} & \dots & \px{x_d}{\xi_1} \\
			\px{x_1}{\xi_2} & \px{x_2}{\xi_2} & \dots & \px{x_d}{\xi_2} \\
			\vdots & \vdots & \ddots & \vdots \\
			\px{x_1}{\xi_d} & \px{x_2}{\xi_d} & \dots & \px{x_d}{\xi_d}
		\end{bmatrix} \quad \mathrm{and} \quad J_n = |\mathbf{G}_n| 
	\end{equation} 
	
	\begin{equation}
		\hat{\nabla} = \begin{bmatrix}
			\px{}{\xi_1} \\
			\px{}{\xi_2} \\
			\vdots
		\end{bmatrix}
	\end{equation}
	
	\begin{equation}
		\px{u}{t}  + \px{f}{x} = 0
	\end{equation}
	\begin{equation}
		u^\delta = \bigcup^N_{n=1}u^\delta_n \approx u \quad \mathrm{and} \quad f^\delta = \bigcup^N_{n=1}f^\delta_n \approx f.
	\end{equation}
	
	\begin{equation}
		\px{\hud}{t} + \px{\hfd}{\xi} = 0
	\end{equation}
	
	\begin{equation}
		\hud = J_n u^\delta \quad \mathrm{and} \quad \hfd = J_n f^\delta 
	\end{equation}
	
	\begin{equation}
		\hud = \sum^p_{i=0}\hud_i(\xi) l_i(\xi)
	\end{equation}
	\begin{equation}
		l_i = \prod^p_{\substack{j=0\\j\ne i}}\bigg(\frac{\xi-\xi_j}{\xi_i-\xi_j}\bigg).
	\end{equation}
	
	\begin{equation}
		\hfD = \sum^{p}_{i=0} \hfD_il_i(\xi)
	\end{equation}
	
	\begin{align}
		h_L(-1) = 1 \quad &\mathrm{and} \quad h_L(1) = 0; \\
		h_R(-1) = 0 \quad &\mathrm{and} \quad h_R(1) = 1.
	\end{align}
	\begin{equation}
		\hfC = \Big(\hfI_L - \hfD_L\Big)h_L(\xi) + \Big(\hfI_R - \hfD_R\Big)h_R(\xi)
	\end{equation}
	\begin{equation}
		\hfd = \hfD + \hfC = \hfD(\xi) + \Big(\hfI_L - \hfD_L\Big)h_L(\xi) + \Big(\hfI_R - \hfD_R\Big)h_R(\xi)
	\end{equation}
	
	\begin{equation}
		\hfd = \hfD + \hfC = \sum^{p}_{i=0}\hfD_il_i(\xi) + \Big(\hfI_L - \hfD_L\Big)h_L(\xi) + \Big(\hfI_R - \hfD_R\Big)h_R(\xi)
	\end{equation}
	
	\begin{equation}
		\px{\hfd}{\xi} = \sum^{p}_{i=0}\hfD_i\dx{l_i(\xi)}{\xi} + \Big(\hfI_L - \hfD_L\Big)\dx{h_L(\xi)}{\xi} + \Big(\hfI_R - \hfD_R\Big)\dx{h_R(\xi)}{\xi}
	\end{equation}

\end{document}
